Fomega/Algorithm.lean
@@ -3,149 +3,136 @@ import Fomega.Proof
 import Fomega.Basic
 
 namespace Fomega
+  partial def normalize (t : Term) : Term :=
+    let t' := t.compl
+    if t' == t then t else normalize t'
 
   @[simp]
-  abbrev CheckArgs : JudgmentVariant -> Type
-  | .prf => Term
-  | .wf => Unit
+  def is_kind : Term -> Option Const
+  | .const K => .some K
+  | _ => .none
 
   @[simp]
-  abbrev CheckRets : JudgmentVariant -> Type
-  | .prf => Option Term
-  | .wf => Option Unit
-
-  partial def normalize : Term -> Term := by sorry
-
-  def is_kind : Term -> Option Const := by sorry
-
-  def is_type : Term -> Option Unit := by sorry
+  def is_type : Term -> Option Unit
+  | .const .type => .some ()
+  | _ => .none
 
   def is_dom : Const -> Const -> Option Unit := by sorry
 
-  def is_pi : Term -> Option (Term × Term) := by sorry
+  def is_pi (t : Term) : Option (Term × Term) :=
+    match normalize t with
+    | .all A B => .some (A, B)
+    | _ => .none
 
-  def is_times : Term -> Option (Term × Term) := by sorry
+  def is_times (t : Term) : Option (Term × Term) :=
+    match normalize t with
+    | .times A B => .some (A, B)
+    | _ => .none
 
-  def is_unit : Term -> Option Unit := by sorry
+  def is_unit (t : Term) : Option Unit :=
+    match normalize t with
+    | .unit_ty => .some ()
+    | _ => .none
 
-  def conv : Term -> Term -> Option Unit := by sorry
+  def conv (a b : Term) : Option Unit :=
+    if normalize a == normalize b then .some () else .none
 
-  def check_witness : (k : JudgmentVariant) -> Ctx Term -> CheckArgs k -> CheckRets k
-  | .wf, _, () => .some .unit
-  | .prf, _, t => .some t
+  inductive Depth where
+  | term | type | kind
 
-  instance inst_Inhabited_check_def : Inhabited ((k : JudgmentVariant) -> Ctx Term -> CheckArgs k -> CheckRets k) where
-    default := check_witness
-
-  @[simp]
-  def check : (k : JudgmentVariant) -> Ctx Term -> CheckArgs k -> CheckRets k
-  | .wf, [], () => .some .unit
-  | .wf, .cons A Γ, () => do
-    let Ak <- check .prf Γ A
-    let _ <- check .wf Γ ()
-    let _ <- is_kind Ak
-    .some ()
-  | .prf, _, □ => .none
-  | .prf, Γ, ★ => do
-    let _ <- check .wf Γ ()
-    .some □
-  | .prf, Γ, #x => do
-    let _ <- check .wf Γ ()
-    .some (Γ d@ x)
-  | .prf, Γ, Π[A] B => do
-    let Ak <- check .prf Γ A
+  def infer : Depth -> Ctx Term -> Term -> Option Term
+  | .kind, Γ, ★ => .some □
+  | .term, Γ, #x => .some (Γ d@ x)
+  | .type, Γ, #x => .some (Γ d@ x)
+  | Γ, Π[A] B => do
+    let Ak <- infer Γ A
     let Ak <- is_kind Ak
-    let Bk <- check .prf (A::Γ) B
+    let Bk <- infer (A::Γ) B
     let Bk <- is_kind Bk
     let _ <- is_dom Ak Bk
     .some (.const Bk)
-  | .prf, Γ, `λ[A] t => do
-    let Ak <- check .prf Γ A
+  | Γ, `λ[A] t => do
+    let Ak <- infer Γ A
     let Ak <- is_kind Ak
-    let B <- check .prf (A::Γ) t
-    let Bk <- check .prf (A::Γ) B
+    let B <- infer (A::Γ) t
+    let Bk <- infer (A::Γ) B
     let Bk <- is_kind Bk
     let _ <- is_dom Ak Bk
     .some (Π[A] B)
-  | .prf, Γ, f `@ a => do
-    let T <- check .prf Γ f
+  | Γ, f `@ a => do
+    let T <- infer Γ f
     let (A, B) <- is_pi T
-    let A' <- check .prf Γ a
+    let A' <- infer Γ a
     let _ <- conv A A'
     .some (B β[a])
-  | .prf, Γ , A ⊗ B => do
-    let Ak <- check .prf Γ A
+  | Γ , A ⊗ B => do
+    let Ak <- infer Γ A
     let _ <- is_type Ak
-    let Bk <- check .prf Γ B
+    let Bk <- infer Γ B
     let _ <- is_type Bk
     .some ★
-  | .prf, Γ, (.pair t s) => do
-    let A <- check .prf Γ t
-    let Ak <- check .prf Γ A
+  | Γ, (.pair t s) => do
+    let A <- infer Γ t
+    let Ak <- infer Γ A
     let _ <- is_type Ak
-    let B <- check .prf Γ s
-    let Bk <- check .prf Γ B
+    let B <- infer Γ s
+    let Bk <- infer Γ B
     let _ <- is_type Bk
     .some (A ⊗ B)
-  | .prf, Γ, (.fst t) => do
-    let T <- check .prf Γ t
+  | Γ, (.fst t) => do
+    let T <- infer Γ t
     let (A, _) <- is_times T
     .some A
-  | .prf, Γ, (.snd t) => do
-    let T <- check .prf Γ t
+  | Γ, (.snd t) => do
+    let T <- infer Γ t
     let (_, B) <- is_times T
     .some B
-  | .prf, Γ, .unit_ty => do
-    let _ <- check .wf Γ ()
-    .some ★
-  | .prf, Γ, .unit => do
-    let _ <- check .wf Γ ()
-    .some (U)
-  | .prf, Γ, (.unit_rec d u t) => do
-    let _ <- check .prf Γ d
-    let T <- check .prf Γ u
+  | Γ, .unit_ty => .some ★
+  | Γ, .unit => .some (U)
+  | Γ, (.unit_rec d u t) => do
+    let _ <- infer Γ d
+    let T <- infer Γ u
     let _ <- is_unit T
-    let A <- check .prf Γ t
-    let Ak <- check .prf Γ A
+    let A <- infer Γ t
+    let Ak <- infer Γ A
     let _ <- is_type Ak
     .some A
-  decreasing_by
-    repeat sorry
+  | _, _, _ => .none
 
-  @[simp]
-  abbrev CheckSoundType (Γ : Ctx Term) : (v : JudgmentVariant) -> CheckArgs v -> CheckRets v -> Prop
-  | .prf => λ t r => ∀ A, r = .some A -> Γ ⊢ t : A
-  | .wf => λ _ r => r = .some () -> ⊢ Γ
+  -- @[simp]
+  -- abbrev CheckSoundType (Γ : Ctx Term) : (v : JudgmentVariant) -> CheckArgs v -> CheckRets v -> Prop
+  -- | .prf => λ t r => ∀ A, r = .some A -> Γ ⊢ t : A
+  -- | .wf => λ _ r => r = .some () -> ⊢ Γ
 
-  theorem check_sound : check v Γ t = r -> CheckSoundType Γ v t r := by
-  intro h
-  induction v, Γ, t, r using check.induct <;> simp at *
-  case _ => intro h2; constructor
-  case _ ih1 ih2 =>
-    intro h1; subst h1
-    rw [Option.bind_eq_some] at h
-    cases h; case _ v1 h =>
-    cases h; case _ h1 h2 =>
-    rw [Option.bind_eq_some] at h2
-    cases h2; case _ v2 h2 =>
-    cases h2; case _ h2 h3 =>
-    rw [Option.bind_eq_some] at h3
-    cases h3; case _ v3 h3 =>
-    replace ih1 := ih1 _ h1
-    replace ih2 := ih2 h2
-    sorry
-  case _ => sorry
-  case _ => sorry
-  case _ => sorry
-  case _ => sorry
-  case _ => sorry
-  case _ => sorry
-  case _ => sorry
-  case _ => sorry
-  case _ => sorry
-  case _ => sorry
-  case _ => sorry
-  case _ => sorry
-  case _ => sorry
+  -- theorem check_sound : check v Γ t = r -> CheckSoundType Γ v t r := by
+  -- intro h
+  -- induction v, Γ, t, r using check.induct <;> simp at *
+  -- case _ => intro h2; constructor
+  -- case _ ih1 ih2 =>
+  --   intro h1; subst h1
+  --   rw [Option.bind_eq_some] at h
+  --   cases h; case _ v1 h =>
+  --   cases h; case _ h1 h2 =>
+  --   rw [Option.bind_eq_some] at h2
+  --   cases h2; case _ v2 h2 =>
+  --   cases h2; case _ h2 h3 =>
+  --   rw [Option.bind_eq_some] at h3
+  --   cases h3; case _ v3 h3 =>
+  --   replace ih1 := ih1 _ h1
+  --   replace ih2 := ih2 h2
+  --   sorry
+  -- case _ => sorry
+  -- case _ => sorry
+  -- case _ => sorry
+  -- case _ => sorry
+  -- case _ => sorry
+  -- case _ => sorry
+  -- case _ => sorry
+  -- case _ => sorry
+  -- case _ => sorry
+  -- case _ => sorry
+  -- case _ => sorry
+  -- case _ => sorry
+  -- case _ => sorry
 
 end Fomega
