Fomega/Algorithm/Soundness.lean
@@ -1,0 +1,22 @@
+import Fomega.Proof
+import Fomega.Basic
+import Fomega.Algorithm
+
+namespace Fomega
+
+  theorem infer_kind_sound :
+    infer_kind Γ t = .some A ->
+    ⊢ Γ ->
+    Γ ⊢ t : A
+  := by
+    intro h1 h2
+    induction Γ, t using infer_kind.induct generalizing A
+    case _ => sorry
+    case _ => sorry
+    case _ => sorry
+    case _ => sorry
+    case _ => sorry
+    case _ => sorry
+    case _ => sorry
+
+end Fomega
