Fomega/Basic.lean
@@ -1,7 +1,6 @@
 
 import Fomega.Basic.Classification
 import Fomega.Basic.Inversion
-import Fomega.Basic.Strengthen
 import Fomega.Basic.Substitution
 import Fomega.Basic.Weaken
 import Fomega.Basic.Derivations
