Fomega/Term/Definition.lean
@@ -1,0 +1,34 @@
+
+namespace Fomega
+  inductive Const : Type where
+  | kind | type
+  deriving Repr
+
+  inductive Term : Type where
+  | var : Nat -> Term
+  | const : Const -> Term
+  | app : Term -> Term -> Term
+  | lam : Term -> Term -> Term
+  | all : Term -> Term -> Term
+  | pair : Term -> Term -> Term
+  | fst : Term -> Term
+  | snd : Term -> Term
+  | times : Term -> Term -> Term
+  | unit : Term
+  | unit_ty : Term
+  | unit_rec : Term -> Term -> Term -> Term
+  deriving Repr
+
+  notation "★" => Term.const Const.type
+  notation "□" => Term.const Const.kind
+  infixl:15 " `@ " => Term.app
+  notation "`λ[" A "]" t:50 => Term.lam A t
+  notation "Π[" A "]" t:50 => Term.all A t
+  infixl:15 "⊗" => Term.times
+  notation "(u)" => Term.unit
+  notation "(U)" => Term.unit_ty
+  prefix:max "#" => Term.var
+
+  instance instInhabited_Term : Inhabited Term where
+  default := ★
+end Fomega
