Fomega/Term/Equality.lean
@@ -1,0 +1,44 @@
+import Fomega.Term.Definition
+
+namespace Fomega.Const
+  @[simp]
+  def beq : Const -> Const -> Bool
+  | .kind, .kind => true
+  | .type, .type => true
+  | _, _ => false
+
+  @[simp]
+  instance instBEq_Const : BEq Const where
+    beq := Const.beq
+
+  instance instLawfulBEq_Const : LawfulBEq Const where
+    eq_of_beq := by intro a b h; cases a <;> cases b <;> simp at * <;> simp [*]
+    rfl := by intro a; cases a <;> simp
+end Fomega.Const
+
+namespace Fomega.Term
+  def beq : Term -> Term -> Bool
+  | var x, var y => x == y
+  | const k1, const k2 => k1 == k2
+  | app x1 x2, app y1 y2 => beq x1 y1 && beq x2 y2
+  | lam x1 x2, lam y1 y2 => beq x1 y1 && beq x2 y2
+  | all x1 x2, all y1 y2 => beq x1 y1 && beq x2 y2
+  | pair x1 x2, pair y1 y2 => beq x1 y1 && beq x2 y2
+  | fst x, fst y => beq x y
+  | snd x, snd y => beq x y
+  | times x1 x2, times y1 y2 => beq x1 y1 && beq x2 y2
+  | unit, unit => true
+  | unit_ty, unit_ty => true
+  | unit_rec x1 x2 x3, unit_rec y1 y2 y3 =>
+    beq x1 y1 && beq x2 y2 && beq x3 y3
+  | _, _ => false
+
+  @[simp]
+  instance instBEq_Term : BEq Term where
+    beq := Term.beq
+
+  instance instLawfulBEq_Term : LawfulBEq Term where
+    eq_of_beq := by sorry
+    rfl := by sorry
+
+end Fomega.Term
