Fomega/Term/Substitution.lean
@@ -1,0 +1,101 @@
+import Common.Substitution
+import Fomega.Term.Definition
+
+namespace Fomega.Term
+  @[simp]
+  def smap (lf : Subst.Lift Term) (f : Nat -> Subst.Action Term) : Term -> Term
+  | var x =>
+    match f x with
+    | .re y => var y
+    | .su t => t
+  | const k => const k
+  | app t1 t2 => app (smap lf f t1) (smap lf f t2)
+  | lam A t => lam (smap lf f A) (smap lf (lf f) t)
+  | all t1 t2 => all (smap lf f t1) (smap lf (lf f) t2)
+  | pair t1 t2 => pair (smap lf f t1) (smap lf f t2)
+  | fst t => fst (smap lf f t)
+  | snd t => snd (smap lf f t)
+  | times t1 t2 => times (smap lf f t1) (smap lf f t2)
+  | unit => unit
+  | unit_ty => unit_ty
+  | unit_rec t1 t2 t3 => unit_rec (smap lf f t1) (smap lf f t2) (smap lf f t3)
+
+  @[simp↓]
+  instance substType_Term : SubstitutionType Term where
+    smap := Term.smap
+
+  @[simp↓]
+  theorem subst_var : [σ]#x = match σ x with | .re y => #y | .su t => t := by
+  unfold Subst.apply; simp
+
+  @[simp] -- 0[s.σ ] = s
+  theorem subst_var_replace : [.su s :: σ]var 0 = s := by simp
+
+  @[simp] -- 0[s.σ ] = s
+  theorem subst_var_rename : [.re k :: σ]var 0 = var k := by simp
+
+  @[simp]
+  theorem subst_const  : [σ]const k = const k := by unfold Subst.apply; simp
+
+  @[simp]
+  theorem subst_app : [σ](app t1 t2) = app ([σ]t1) ([σ]t2) := by unfold Subst.apply; simp
+
+  @[simp]
+  theorem subst_lam : [σ](lam A t) = lam ([σ]A) ([^σ]t) := by unfold Subst.apply; simp
+
+  @[simp]
+  theorem subst_all : [σ]all t1 t2 = all ([σ]t1) ([^σ]t2) := by unfold Subst.apply; simp
+
+  @[simp]
+  theorem subst_pair : [σ]pair t1 t2 = pair ([σ]t1) ([σ]t2) := by unfold Subst.apply; simp
+
+  @[simp]
+  theorem subst_fst : [σ]fst t = fst ([σ]t) := by unfold Subst.apply; simp
+
+  @[simp]
+  theorem subst_snd : [σ]snd t = snd ([σ]t) := by unfold Subst.apply; simp
+
+  @[simp]
+  theorem subst_times : [σ]times t1 t2 = times ([σ]t1) ([σ]t2) := by unfold Subst.apply; simp
+
+  @[simp]
+  theorem subst_unit : [σ]unit = unit := by unfold Subst.apply; simp
+
+  @[simp]
+  theorem subst_unit_ty : [σ]unit_ty = unit_ty := by unfold Subst.apply; simp
+
+  @[simp]
+  theorem subst_unit_rec :
+    [σ]unit_rec t1 t2 t3 = unit_rec ([σ]t1) ([σ]t2) ([σ]t3)
+  := by unfold Subst.apply; simp
+
+  theorem apply_id {t : Term} : [I]t = t := by
+  have lem : ^I = @I Term := by
+    funext; case _ x =>
+    cases x; all_goals (unfold Subst.lift; unfold I; simp)
+  induction t
+  all_goals (simp at * <;> try simp [*])
+
+  theorem apply_stable {r : Ren} {σ : Subst Term}
+    : r.to = σ -> Ren.apply r = Subst.apply σ
+  := by
+  intro h; funext; case _ x =>
+    unfold Ren.apply; simp at *
+    unfold Ren.to; simp
+    induction x generalizing r σ <;> simp at *
+    any_goals simp [*]
+    case _ x => rw [<-h]; unfold Ren.to; simp
+    any_goals
+      rw [Subst.lift_lemma, <-h]
+      unfold Ren.fro; simp
+
+  theorem apply_compose {s : Term} {σ τ : Subst Term} : [τ][σ]s = [τ ⊙ σ]s := by
+  solve_compose Term, apply_stable, s, σ, τ
+
+  instance substTypeLaws_Term : SubstitutionTypeLaws Term where
+    apply_id := Term.apply_id
+    apply_compose := Term.apply_compose
+    apply_stable := Term.apply_stable
+
+
+end Fomega.Term
