Main.lean
@@ -1,5 +1,4 @@
 
 import Common
-import WCCC
 
 def main := IO.println "Hello, World!"
